src/dafny/BinaryOperations.md
@@ -5,9 +5,9 @@ The `Binary Operations` module defines a number of properties of binary operatio
 
 Properties of binary operations `bop`:
 - Associative: `bop(bop(x, y), z) == bop(x, bop(y, z))`
-- Unital: `bop(e, x) == x == bop(x, e)`
+- Unital: `bop(unit, x) == x == bop(x, unit)`
 - Abelian: `bop(x, y) == bop(y, x)`
-- Inverse: `bop(x, inv(x)) == e == bop(inv(x), x)`
+- Inverse: `bop(x, inverse(x)) == unit == bop(inverse(x), x)`
 - Distributive: `bop2(bop1(x, y), z) == bop1(bop2(x, z), bop2(y, z))` and `bop2(x, bop1(y, z)) == bop1(bop2(x, y), bop2(x, z))`
 - Monoid: Associative, Unital
 - Group: Monoid, Inverse
